\section{Teorinės dalies aprašymas}

\subsection{Teiloro skleidinys}

Teiloro begalinis skleidinys

\[\lim_{x \to a} f(x) = f(a) + \frac{f'(a)}{1!}(x-a)+\frac{f''(a)}{2!}(x-a)^2 + \frac{f'''(a)}{3!}(x-a)^3 + ...\]

\[\lim_{x \to a} f(x) = \sum_{n=0}^{\infty} \frac{f^{(n)}(a)}{n!}(x-a)^n\]

Teiloro baigtinis skleidinys

\[\lim_{x \to a} f(x) = f(a) + \frac{f'(a)}{1!}(x-a)+\frac{f''(a)}{2!}(x-a)^2 + ... + \frac{f^{(n)}(a)}{n!}(x-a)^n + r_n(x) \]

\[\lim_{x \to a} f(x) = \sum_{k=0}^{n} \frac{f^{(k)}(a)}{k!}(x-a)^k + r_n(x)\]

$e^x$ riba

\[\lim_{x \to a} e^x= e^a + \frac{e^a}{1!} (x-a) + \frac{e^a}{2!}(x-a)^2 + \frac{e^a}{3!}(x-a)^3 + ... \]

Kai $a = 0$, tai: 
\[\lim_{x \to 0} e^x= e^0 +  \frac{e^0}{1!} (x-0) + \frac{e^0}{2!} (x-0)^2 + \frac{e^0}{3!} (x-0)^3 + ... = 1 + x + \frac{x^2}{2} + \frac{x^3}{6} + ... \]

$e^x$ riba

\[\lim_{x \to a} e^x= e^a + \frac{e^a}{1!} (x-a) + \frac{e^a}{2!}(x-a)^2 + \frac{e^a}{3!}(x-a)^3 + ... \]

Kai $a = 0$, tai: 
\[\lim_{x \to 0} e^x= e^0 +  \frac{e^0}{1!} (x-0) + \frac{e^0}{2!} (x-0)^2 + \frac{e^0}{3!} (x-0)^3 + ... = 1 + x + \frac{x^2}{2} + \frac{x^3}{6} + ... \]

$(1+x)^k$ riba

\[\lim_{x \to a} (1+x)^k =\]
\[=(1+x)^k + \frac{k(1+a)^{k-1}}{1!} (x-a) + \frac{k(k-1)(1+a)^{k-2}}{2!}(x-a)^2 + \frac{{k(k-1)(k-2)(1+a)^{k-3}}}{3!}(x-a)^3 + ... \]

Kai $a = 0$, tai: 

\[\lim_{x \to 0} (1+x)^k =\]
\[=(1)^k + \frac{k(1)^{k-1}}{1!} (x-0) + \frac{k(k-1)(1)^{k-2}}{2!}(x-0)^2 + \frac{{k(k-1)(k-2)(1)^{k-3}}}{3!}(x-0)^3 + ...  = \]
\[=1 + kx + \frac{k(k-1)}{2}x^2 + \frac{{k(k-1)(k-2)}}{6}x^3 + ...  = \]

$\arctan(x)$ riba

\[\lim_{x \to a} \arctan(x) = \arctan(a) + \frac{\frac{1}{a^2+1}}{1!}(x-a) + \frac{\frac{-2a}{(a^2+1)^2}}{2!}(x-a)^2 + \frac{\frac{6a^2-2}{(a^2+1)^3}}{3!}(x-a)^3 \]

Kai $a = 0$, tai: 

\[\lim_{x \to 0} \arctan(x) = \arctan(0) + \frac{\frac{1}{0^2+1}}{1!}(x-0) + \frac{\frac{-2*0}{(0^2+1)^2}}{2!}(x-0)^2 + \frac{\frac{6*0^2-2}{(0^2+1)^3}}{3!}(x-0)^3 =\]
\[= 0 + x + 0 + \frac{1}{3} x^3 +... = x - \frac{x^3}{3} + \frac{x^5}{5} - ... \]




\subsection{Laipsnių eilutės}


\[\sum_{n=0}^{\infty} a_n(x_n)^n = a_0 + a_1 x + a_2 x^2 + ...\]

\[\sum_{m=1}^{k} b_m(x_m)^{-m} = b_1 x^{-1} + b_2 x^{-2} + ... + b_k x^{-k}\]

\[\sum_{n=0}^{\infty} a_n(x_n)^n + \sum_{m=-1}^{-k} a_m(x_m)^m = \sum_{i=-k}^{\infty} a_i(x_i)^i  = a_{-k} x^{-k} + ... + a_{-1} x^{-1} + a_0 + a_1 x + ... \]

\[c_n x^n = a_n(x_n)^n + a_{n-1}x^{n-1} \times b_{1}{x} + a_{n+1}(x_{n+1}) \times b_{-1}x^{-1} + ...\]

\[f(a) + \frac{f'(a)}{1!}(x)+\frac{f''(a)}{2!}(x)^2 + +\frac{f'''(a)}{3!}(x)^3 + ...\]

\[f(a) + \frac{f'(a)}{1!}(S-a)+\frac{f''(a)}{2!}(S-a)^2 + \frac{f'''(a)}{3!}(S-a)^3 + ...\]

$P = (S - a_0)/x$

$S - a_0 = P \times x$

\[f(a) + \frac{f'(a)}{1!}(Px)+\frac{f''(a)}{2!}(Px)^2 + +\frac{f'''(a)}{3!}(Px)^3 + ...\]

\[ g(a,n) = \frac{f^{(n)}(a)}{n!}\]